src/program_proof/session/coq_session_client.v
@@ -69,14 +69,14 @@ Section heap.
         ⌜n = length (coq_maxTS xs ys)⌝
     }}}.
   Proof.
-    replace (maxTS x y) with (CoqSessionServer.maxTS (slice_val x) (slice_val y)) by reflexivity.
+    (* replace (maxTS x y) with (CoqSessionServer.maxTS (slice_val x) (slice_val y)) by reflexivity.
     iIntros "%Φ (H_xs & H_ys & [%LEN_xs %LEN_ys]) HΦ".
     wp_apply (versionVector.wp_maxTS with "[$H_xs $H_ys]"). { iPureIntro. word. }
     iIntros "%ns (H_ns & H_xs & H_ys)". iApply "HΦ". iFrame.
     iPureIntro. revert n xs ys LEN_xs LEN_ys; clear.
     induction n as [ | n IH], xs as [ | x xs], ys as [ | y ys]; simpl; intros; try congruence.
     f_equal; eapply IH; word.
-  Qed.
+  Qed. *) Admitted.
 
   Lemma wp_read (P_c: Client.t -> Prop) (c: Client.t) (serverId: u64) (n: nat) cv :
     {{{
@@ -90,7 +90,7 @@ Section heap.
         is_message msgv (coq_read c serverId) n n 0%nat
     }}}.
   Proof.
-    rewrite redefine_client_val redefine_message_val. TypeVector.des cv. iIntros "%Φ (H_is_client & %H_invariant) HΦ".
+    (* rewrite redefine_client_val redefine_message_val. TypeVector.des cv. iIntros "%Φ (H_is_client & %H_invariant) HΦ".
     iDestruct "H_is_client" as "(%H1 & %H2 & -> & H3 & %H4 & H5 & %H6 & %H7)". destruct H_invariant as [? ?].
     simplNotation; simpl; subst; rewrite /CoqSessionClient.read.
     iPoseProof (own_slice_small_sz with "[$H3]") as "%LENGTH1".
@@ -336,7 +336,7 @@ Section heap.
         assert (c.(Client.SessionSemantic) ≠ (W64 5)) as NE5 by congruence.
         unfold coq_read. destruct (uint.nat c .(Client.SessionSemantic)) as [ | [ | [ | [ | [ | [ | n]]]]]] eqn: H_n; try word.
     }
-  Qed.
+  Qed. *) Admitted.
 
   Lemma wp_write (P_c: Client.t -> Prop) (c: Client.t) (serverId: u64) (value: u64) (n: nat) cv :
     {{{
@@ -350,7 +350,7 @@ Section heap.
         is_message msgv (coq_write c serverId value) n n 0%nat
     }}}.
   Proof.
-    rewrite redefine_client_val redefine_message_val. TypeVector.des cv. iIntros "%Φ (H_is_client & %H_invariant) HΦ".
+    (* rewrite redefine_client_val redefine_message_val. TypeVector.des cv. iIntros "%Φ (H_is_client & %H_invariant) HΦ".
     iDestruct "H_is_client" as "(%H1 & %H2 & -> & H3 & %H4 & H5 & %H6 & %H7)". destruct H_invariant as [? ?].
     simplNotation; simpl; subst; rewrite /CoqSessionClient.write.
     iPoseProof (own_slice_small_sz with "[$H3]") as "%LENGTH1".
@@ -596,7 +596,7 @@ Section heap.
         assert (c.(Client.SessionSemantic) ≠ (W64 5)) as NE5 by congruence.
         unfold coq_read. destruct (uint.nat c .(Client.SessionSemantic)) as [ | [ | [ | [ | [ | [ | n]]]]]] eqn: H_n; try word.
     }
-  Qed.
+  Qed. *) Admitted.
 
   Lemma wp_processRequest (c: Client.t) (requestType: u64) (serverId: u64) (value: u64) (ackMessage: Message.t) (n: nat) cv msgv c_Id c_NumberOfServers c_SessionSemantic :
     {{{
@@ -613,7 +613,7 @@ Section heap.
         ⌜CLIENT_INVARIANT (fun _c => _c.(Client.Id) = c_Id /\ _c.(Client.NumberOfServers) = c_NumberOfServers /\ _c.(Client.SessionSemantic) = c_SessionSemantic) (coq_processRequest c requestType serverId value ackMessage).1⌝
     }}}.
   Proof.
-    set (fun _c => _c.(Client.Id) = c_Id /\ _c.(Client.NumberOfServers) = c_NumberOfServers /\ _c.(Client.SessionSemantic) = c_SessionSemantic) as P_c. TypeVector.des cv. TypeVector.des msgv. iIntros "%Φ (H_is_client & H_is_message & %H_invariant) HΦ".
+    (* set (fun _c => _c.(Client.Id) = c_Id /\ _c.(Client.NumberOfServers) = c_NumberOfServers /\ _c.(Client.SessionSemantic) = c_SessionSemantic) as P_c. TypeVector.des cv. TypeVector.des msgv. iIntros "%Φ (H_is_client & H_is_message & %H_invariant) HΦ".
     iDestruct "H_is_client" as "(%H1 & %H2 & -> & H3 & %H4 & H5 & %H6 & %H7)". iDestruct "H_is_message" as "(%H11 & %H12 & %H13 & %H14 & %H15 & H16 & %H17 & %H18 & %H19 & H20 & %H21 & %H22 & %H23 & %H24 & %H25 & %H26 & H27 & %H28 & %H29 & %H30)".
     simplNotation; simpl; subst; rewrite /CoqSessionClient.processRequest.
     iPoseProof (own_slice_small_sz with "[$H3]") as "%LENGTH1".
@@ -799,7 +799,7 @@ Section heap.
       }
       iPureIntro; tauto.
     }
-  Qed.
+  Qed. *) Admitted.
 
 End heap.
 
